Rename exec_prefix to exec
This is the counter-free version.

src/Spec/ConcurExec.v
@@ -99,22 +99,21 @@ Section Proc.
   .
 
 
-  (* TODO: rename to exec *)
-  Inductive exec_prefix : State -> threads_state Op -> trace -> Prop :=
+  Inductive exec : State -> threads_state Op -> trace -> Prop :=
 
   | ExecOne : forall T tid tid' (ts : threads_state Op) trace p s s' evs result spawned,
     ts tid = @Proc Op T p ->
     ts tid' = NoProc ->
     exec_tid tid s p s' result spawned evs ->
-    exec_prefix s' (thread_upd (thread_upd ts tid' spawned) tid
+    exec s' (thread_upd (thread_upd ts tid' spawned) tid
               match result with
               | inl _ => NoProc
               | inr p' => Proc p'
               end) trace ->
-    exec_prefix s ts (prepend tid evs trace)
+    exec s ts (prepend tid evs trace)
 
   | ExecStop : forall (ts : threads_state Op) s,
-    exec_prefix s ts TraceEmpty.
+    exec s ts TraceEmpty.
 
   Theorem ExecPrefixOne
        : forall (T : Type)
@@ -125,13 +124,13 @@ Section Proc.
          thread_get ts tid = Proc p ->
          thread_get ts tid' = NoProc ->
          exec_tid tid s p s' result spawned evs ->
-         exec_prefix s'
+         exec s'
            (thread_upd (thread_upd ts tid' spawned) tid
              (match result with
               | inl _ => NoProc
               | inr p' => Proc p'
               end)) tr ->
-         exec_prefix s ts (prepend tid evs tr).
+         exec s ts (prepend tid evs tr).
   Proof.
     intros.
     eapply ExecOne; eauto.
@@ -241,7 +240,7 @@ Section Proc.
 
 End Proc.
 
-Hint Constructors exec_prefix.
+Hint Constructors exec.
 Hint Constructors exec_any.
 Hint Resolve exec_tid_exec_others.
 Hint Resolve exec_others_exec_any.
@@ -354,10 +353,10 @@ Ltac cmp_ts tid1 tid2 :=
   try congruence;
   autorewrite with t in *.
 
-Local Lemma exec_prefix_ts_eq : forall Op State (op_step: OpSemantics Op State) s ts ts' tr,
-    exec_prefix op_step s ts' tr ->
+Local Lemma exec_ts_eq : forall Op State (op_step: OpSemantics Op State) s ts ts' tr,
+    exec op_step s ts' tr ->
     ts = ts' ->
-    exec_prefix op_step s ts tr.
+    exec op_step s ts tr.
 Proof.
   propositional.
 Qed.
@@ -366,13 +365,13 @@ Qed.
 forms) *)
 Ltac abstract_ts :=
   match goal with
-  | |- exec_prefix _ _ ?ts _ => eapply exec_prefix_ts_eq
+  | |- exec _ _ ?ts _ => eapply exec_ts_eq
   end.
 
-Local Lemma exec_prefix_tr_eq : forall Op State (op_step: OpSemantics Op State) s ts tr tr',
-    exec_prefix op_step s ts tr' ->
+Local Lemma exec_tr_eq : forall Op State (op_step: OpSemantics Op State) s ts tr tr',
+    exec op_step s ts tr' ->
     tr = tr' ->
-    exec_prefix op_step s ts tr.
+    exec op_step s ts tr.
 Proof.
   propositional.
 Qed.
@@ -381,5 +380,5 @@ Qed.
 prepend/list append) *)
 Ltac abstract_tr :=
   match goal with
-  | |- exec_prefix _ _ _ ?tr => eapply exec_prefix_tr_eq
+  | |- exec _ _ _ ?tr => eapply exec_tr_eq
   end.
