src/Spec/Abstraction.v
@@ -72,8 +72,8 @@ Section StateAbstraction.
   Theorem trace_incl_abs :
     forall s1 s2 (ts : threads_state opLoT) tr,
       absR s1 s2 ->
-      exec_prefix lo_step s1 ts tr ->
-      exec_prefix hi_step s2 ts tr.
+      exec lo_step s1 ts tr ->
+      exec hi_step s2 ts tr.
   Proof.
     intros.
     generalize dependent s2.
